- update all elab rules, but needs checking

proof/uni/decl/prop_safety.v
@@ -10,8 +10,8 @@ Require Import systemf.def_ott.
 Require Import systemf.prop_ln.
 
 
-Notation "E ⊢ e : A" :=
-  (f_typing E e A) 
+Notation "Ψ ⊢ e : A" :=
+  (f_typing Ψ e A) 
     (at level 65, e at next level, no associativity) : type_scope.
 
 Fixpoint trans_typ (A : typ) : ftyp :=
@@ -44,7 +44,7 @@ Lemma trans_typ_open_typ_wrt_typ_rec : forall A1 A2 n,
   trans_typ (open_typ_wrt_typ_rec n A2 A1) = open_ftyp_wrt_ftyp_rec n ᵗ⟦ A2 ⟧ ᵗ⟦ A1 ⟧.
 Proof.
   intros A1. induction A1; auto; intros; simpl.
-  - destruct (lt_eq_lt_dec n n0) as [[? | ?] | ?] eqn:E; auto.
+  - destruct (lt_eq_lt_dec n n0) as [[? | ?] | ?] eqn:Ψ; auto.
   - rewrite IHA1_1. rewrite IHA1_2. auto.
   - rewrite IHA1. auto.
   - rewrite IHA1_1. rewrite IHA1_2. auto.
@@ -70,8 +70,8 @@ Qed.
 
 #[local] Hint Resolve trans_typ_lc_ftyp : core.
 
-Theorem trans_env_notin_dom : forall E X,
-  X `notin` dom E -> X `notin` dom (trans_env E).
+Theorem trans_env_notin_dom : forall Ψ X,
+  X `notin` dom Ψ -> X `notin` dom (trans_env Ψ).
 Proof.
   intros Ψ. induction Ψ; auto.
   intros X H. destruct a. destruct d; simpl in *; auto.
@@ -151,12 +151,12 @@ Inductive d_sub_elab : denv -> typ -> typ -> fexp -> Prop :=
                             (fexp_app co2
                                       (fexp_app (fexp_var_b 1)
                                                 (fexp_app co1 (fexp_var_b 0))))))
-  | sub_elab_all : forall (L:vars) (Ψ:denv) (A1 B1:typ) (co:fexp),
-      ( forall X , X \notin L -> s_in X  (open_typ_wrt_typ  A1   (typ_var_f X) ) ) ->
-      ( forall X , X \notin L -> s_in X  (open_typ_wrt_typ  B1   (typ_var_f X) ) ) ->
-      ( forall X , X \notin L -> d_sub_elab  ( X ~ dbind_stvar_empty  ++  Ψ )   (open_typ_wrt_typ  A1   (typ_var_f X) )   (open_typ_wrt_typ  B1   (typ_var_f X) ) co ) ->
-      d_sub_elab Ψ (typ_all A1) (typ_all B1)
-        (fexp_abs (trans_typ (typ_all A1)) (fexp_tabs (fexp_app co (fexp_tapp (fexp_var_b 0) (ftyp_var_b 0)))))
+  | sub_elab_all : forall (L:vars) (Ψ:denv) (A B:typ) (co:fexp),
+      ( forall X , X \notin L -> s_in X  (open_typ_wrt_typ  A   (typ_var_f X) ) ) ->
+      ( forall X , X \notin L -> s_in X  (open_typ_wrt_typ  B   (typ_var_f X) ) ) ->
+      ( forall X , X \notin L -> d_sub_elab  ( X ~ dbind_stvar_empty  ++  Ψ )   (open_typ_wrt_typ  A   (typ_var_f X) )   (open_typ_wrt_typ  B   (typ_var_f X) ) co ) ->
+      d_sub_elab Ψ (typ_all A) (typ_all B)
+        (fexp_abs (trans_typ (typ_all A)) (fexp_tabs (fexp_app co (fexp_tapp (fexp_var_b 0) (ftyp_var_b 0)))))
   | sub_elab_alll : forall (L:vars) (Ψ:denv) (A B T:typ) (co:fexp),
       neq_all B ->
       neq_intersection B ->
@@ -201,45 +201,197 @@ Inductive d_sub_elab : denv -> typ -> typ -> fexp -> Prop :=
         (fexp_abs (trans_typ (typ_union A1 A2)) (fexp_case (fexp_var_b 0) (fexp_app co1 (fexp_var_b 0)) (fexp_app co2 (fexp_var_b 0)))).
 
 
-(* 
+#[local] Hint Constructors d_sub_elab : core.
+#[local] Hint Constructors f_typing : core.
 
 
-
-Notation "E ⊢ A <: B ↪ C" := (d_sub_elab E A B C) (at level 65, A at next level, no associativity) : type_scope.
-
-Hint Constructors d_sub_elab : safety.
-Hint Constructors typing : safety.
-
-Theorem sub_elab_sound: forall E A B C,
-  d_sub_elab E A B C -> d_sub E A B.
+Theorem sub_elab_sound: forall Ψ A B C,
+  d_sub_elab Ψ A B C -> d_sub Ψ A B.
 Proof.
   intros. induction H; eauto.
 Qed.
 
-Theorem sub_elab_complete: forall E A B,
-  d_sub E A B -> exists C, d_sub_elab E A B C.
-Proof.
-  intros. induction H.
-  - eauto with safety.
-  - eauto with safety.
-  - eauto with safety.
-  - eauto with safety.
-  - eauto with safety.
-  - inversion IHd_sub1. inversion IHd_sub2. eauto with safety.
-  - inst_cofinites_by L. inversion H2. eauto with safety.
-    exists (fexp_abs (trans_typ (typ_all A1)) (fexp_tabs (fexp_app x0 (fexp_tapp (fexp_var_b 0) (ftyp_var_b 0))))).
-    apply sub_elab_all with (L := L).
-    + intros. admit.
-    + intros. admit.
-    + intros. admit.
-  - inversion IHd_sub. eauto with safety.
-  - inversion IHd_sub1. inversion IHd_sub2. eauto with safety.
-  - inversion IHd_sub. eauto with safety.
-  - inversion IHd_sub. eauto with safety.
-  - inversion IHd_sub. eauto with safety.
-  - inversion IHd_sub. eauto with safety.
-  - inversion IHd_sub1. inversion IHd_sub2. eauto with safety.
+Notation "Ψ ⊢ A <: B ↪ co" := (d_sub_elab Ψ A B co) (at level 65, A at next level, B at next level, no associativity) : type_scope.
+
+Theorem sub_elab_complete: forall Ψ A B,
+  Ψ ⊢ A <: B -> exists co, Ψ ⊢ A <: B ↪ co.
+Proof with auto.
+  intros. induction H; eauto.
 Admitted.
+
+
+Inductive infabs_elab : denv -> typ -> typ -> typ -> fexp -> Prop := 
+  | infabs_elab_bot : forall (Ψ:denv),
+      d_wf_env Ψ ->
+      infabs_elab Ψ typ_bot typ_top typ_bot
+        (fexp_abs (ftyp_all (ftyp_var_b 0))
+              (fexp_tapp (fexp_var_b 0) (ftyp_arrow ftyp_unit (ftyp_all (ftyp_var_b 0)))))
+  | infabs_elab_arr : forall (Ψ:denv) (A B:typ),
+      d_wf_env Ψ ->
+      d_wf_typ Ψ A ->
+      d_wf_typ Ψ B ->
+      infabs_elab Ψ (typ_arrow A B) A B
+        (fexp_abs (trans_typ (typ_arrow A B)) (fexp_var_b 0))
+  | infabs_elab_all : forall (Ψ:denv) (A B C T:typ) (co:fexp),
+      d_mono_typ Ψ T -> 
+      d_wf_typ Ψ (typ_all A) ->
+      infabs_elab Ψ  (open_typ_wrt_typ  A   T ) B C co ->
+      infabs_elab Ψ (typ_all A) B C
+        (fexp_abs (trans_typ (typ_all A))
+                  (fexp_app co (fexp_tapp (fexp_var_b 0) (trans_typ T))))
+  | infabs_elab_intersection1 : forall (Ψ:denv) (A1 A2 B C:typ) (co:fexp),
+      d_wf_typ Ψ A2 ->
+      infabs_elab Ψ A1 B C co ->
+      infabs_elab Ψ (typ_intersection A1 A2) B C
+        (fexp_abs (trans_typ (typ_intersection A1 A2))
+                  (fexp_app co (fexp_proj1 (fexp_var_b 0))))
+  | infabs_elab_intersection2 : forall (Ψ:denv) (A1 A2 B C:typ) (co:fexp),
+      d_wf_typ Ψ A1 ->
+      infabs_elab Ψ A2 B C co ->
+      infabs_elab Ψ (typ_intersection A1 A2) B C
+        (fexp_abs (trans_typ (typ_intersection A1 A2))
+                  (fexp_app co (fexp_proj2 (fexp_var_b 0))))
+  | infabs_elab_union : forall (Ψ:denv) (A1 A2 B1 C1 B2 C2:typ) (co1 co2:fexp),
+      infabs_elab Ψ A1 B1 C1 co1 ->
+      infabs_elab Ψ A2 B2 C2 co2 ->
+      infabs_elab Ψ (typ_union A1 A2) (typ_intersection B1 B2) (typ_union C1 C2)
+        (fexp_abs (trans_typ (typ_union A1 A2))
+                  (fexp_abs (trans_typ (typ_intersection B1 B2))
+                            (fexp_case (fexp_var_b 1)
+                                      (fexp_inl (fexp_app co1 (fexp_proj1 (fexp_var_b 1))))
+                                      (fexp_inr (fexp_app co2 (fexp_proj2 (fexp_var_b 1))))))).
+
+Notation "Ψ ⊢ A ▹ B → C ↪ co" :=   (infabs_elab Ψ A B C co) 
+  (at level 65, A at next level, B at next level, C at next level, no associativity) : type_scope.
+
+                                    
+Inductive d_inftapp_elab : denv -> typ -> typ -> typ -> fexp -> fexp -> Prop := 
+  | inftapp_elab_bot : forall (Ψ:denv) (B:typ),
+      d_wf_env Ψ -> 
+      d_wf_typ Ψ B ->
+      d_inftapp_elab Ψ typ_bot B typ_bot
+        (fexp_abs (ftyp_all (ftyp_var_b 0)) (fexp_var_b 0))
+        (fexp_abs (ftyp_all (ftyp_var_b 0)) (fexp_var_b 0))
+  | inftapp_elab_all : forall (Ψ:denv) (A B:typ),
+      d_wf_env Ψ -> 
+      d_wf_typ Ψ (typ_all A) ->
+      d_wf_typ Ψ B ->
+      d_inftapp_elab Ψ (typ_all A) B (open_typ_wrt_typ  A   B )  
+        (fexp_abs (trans_typ (typ_all A)) (fexp_var_b 0))
+        (fexp_abs (trans_typ (typ_all A)) (fexp_tapp (fexp_var_b 0) (trans_typ B)))
+  | inftapp_elab_intersection1 : forall (Ψ:denv) (A1 A2 B C1:typ) (co1 co2:fexp),
+      d_wf_typ Ψ A2 ->
+      d_inftapp_elab Ψ A1 B C1 co1 co2 ->
+      d_inftapp_elab Ψ (typ_intersection A1 A2) B C1
+        (fexp_abs (trans_typ (typ_intersection A1 A2))
+                  (fexp_app co1 (fexp_proj1 (fexp_var_b 0))))
+        co2
+  | inftapp_elab_intersection2 : forall (Ψ:denv) (A1 A2 B C2:typ) (co1 co2:fexp),
+      d_wf_typ Ψ A1 ->
+      d_inftapp_elab Ψ A2 B C2 co1 co2 ->
+      d_inftapp_elab Ψ (typ_intersection A1 A2) B C2
+        (fexp_abs (trans_typ (typ_intersection A1 A2))
+                  (fexp_app co1 (fexp_proj2 (fexp_var_b 0))))
+        co2
+  | inftapp_elab_intersection3 : forall (Ψ:denv) (A1 A2 B C1 C2:typ) (co1 co2 co3 co4:fexp),
+      d_inftapp_elab Ψ A1 B C1 co1 co2 ->
+      d_inftapp_elab Ψ A2 B C2 co3 co4 ->
+      d_inftapp_elab Ψ (typ_intersection A1 A2) B (typ_intersection C1 C2)
+        (fexp_abs (trans_typ (typ_intersection A1 A2))
+                  (fexp_pair (fexp_app co2 (fexp_app co1 (fexp_proj1 (fexp_var_b 0))))
+                              (fexp_app co4 (fexp_app co3 (fexp_proj2 (fexp_var_b 0))))))
+        (fexp_abs (trans_typ ((typ_intersection C1 C2))) (fexp_var_b 0))
+  | inftapp_elab_union : forall (Ψ:denv) (A1 A2 B C1 C2:typ) (co1 co2 co3 co4:fexp),
+      d_inftapp_elab Ψ A1 B C1 co1 co2 ->
+      d_inftapp_elab Ψ A2 B C2 co3 co4 ->
+      d_inftapp_elab Ψ (typ_union A1 A2) B (typ_union C1 C2)
+        (fexp_abs (trans_typ (typ_union A1 A2))
+                  (fexp_case (fexp_var_b 0)
+                              (fexp_inl (fexp_app co2 (fexp_app co1 (fexp_var_b 0))))
+                              (fexp_inr (fexp_app co4 (fexp_app co3 (fexp_var_b 0))))))
+        (fexp_abs (trans_typ (typ_union C1 C2)) (fexp_var_b 0)).
+
+Notation "Ψ ⊢ A ○ B ⇒⇒ C ↪ co1 | co2" :=
+    (d_inftapp_elab Ψ A B C co1 co2) 
+      (at level 65, A at next level, B at next level, C at next level, no associativity) : type_scope. 
+
+
+Inductive d_chk_inf_elab : denv -> exp -> typing_mode -> typ -> fexp -> Prop :=
+  | d_chk_inf_elab__inf_var : forall (Ψ:denv) (x:expvar) (A:typ),
+      d_wf_env Ψ ->
+      binds ( x )  ( (dbind_typ A) ) ( Ψ )  ->
+      d_chk_inf_elab Ψ (exp_var_f x) typingmode__inf A
+        (fexp_var_f x)
+  | d_chk_inf_elab__inf_anno : forall (Ψ:denv) (e:exp) (B1:typ) (eᶠ:fexp),
+      d_wf_typ Ψ B1 ->
+      d_chk_inf_elab Ψ e typingmode__chk B1 eᶠ ->
+      d_chk_inf_elab Ψ  ( (exp_anno e B1) )  typingmode__inf B1 eᶠ
+  | d_chk_inf_elab__inf_unit : forall (Ψ:denv),
+      d_wf_env Ψ ->
+      d_chk_inf_elab Ψ exp_unit typingmode__inf typ_unit
+        fexp_unit
+  | d_chk_inf_elab__inf_app : forall (Ψ:denv) (e1 e2:exp) (A B C:typ) (e1ᶠ co e2ᶠ:fexp),
+      d_chk_inf_elab Ψ e1 typingmode__inf A e1ᶠ ->
+      infabs_elab Ψ A B C co ->
+      d_chk_inf_elab Ψ e2 typingmode__chk B e2ᶠ ->
+      d_chk_inf_elab Ψ  ( (exp_app e1 e2) ) typingmode__inf C
+        (fexp_app (fexp_app co e1ᶠ) e2ᶠ)
+  | d_chk_inf_elab__inf_abs_mono : forall (L:vars) (Ψ:denv) (e:exp) (A B:typ) (eᶠ:fexp),
+      d_mono_typ Ψ (typ_arrow A B) ->
+      ( forall x , x \notin  L  -> d_chk_inf_elab  ( x ~ (dbind_typ A)  ++  Ψ )  ( open_exp_wrt_exp e (exp_var_f x) ) typingmode__chk B (open_fexp_wrt_fexp eᶠ (fexp_var_f x)))  ->
+      d_chk_inf_elab Ψ (exp_abs e) typingmode__inf (typ_arrow A B)
+        (fexp_abs (trans_typ A) eᶠ)
+  | d_chk_inf_elab__inf_tabs : forall (L:vars) (Ψ:denv) (e:exp) (A:typ) (eᶠ:fexp),
+      ( forall X , X \notin  L  -> s_in X (open_typ_wrt_typ A (typ_var_f X)))  ->
+      ( forall X , X \notin  L  -> d_chk_inf_elab  ( X ~ dbind_tvar_empty  ++  Ψ ) (exp_anno  ( open_exp_wrt_typ e (typ_var_f X) )  ( open_typ_wrt_typ A (typ_var_f X) ) ) typingmode__chk ( open_typ_wrt_typ A (typ_var_f X) ) (open_fexp_wrt_ftyp eᶠ (ftyp_var_f X)))  ->
+      d_chk_inf_elab Ψ (exp_tabs (exp_anno e A)) typingmode__inf (typ_all A)
+        (fexp_tabs eᶠ)
+  | d_chk_inf_elab__inf_tapp : forall (Ψ:denv) (e:exp) (A B C:typ) (eᶠ co1 co2:fexp),
+      d_wf_typ Ψ B ->
+      d_chk_inf_elab Ψ e typingmode__inf A eᶠ ->
+      d_inftapp_elab Ψ A B C co1 co2 ->
+      d_chk_inf_elab Ψ (exp_tapp e B) typingmode__inf C
+        (fexp_app co2 (fexp_app co1 eᶠ))
+  | d_chk_inf_elab__chk_abs_top : forall (L:vars) (Ψ:denv) (e:exp) (eᶠ:fexp),
+      ( forall x , x \notin  L  -> d_chk_inf_elab  ( x ~ (dbind_typ typ_bot)  ++  Ψ )   ( open_exp_wrt_exp e (exp_var_f x) ) typingmode__chk typ_top (open_fexp_wrt_fexp eᶠ (fexp_var_f x)))  ->
+      d_chk_inf_elab Ψ (exp_abs e) typingmode__chk typ_top fexp_unit
+  | d_chk_inf_elab__chk_abs : forall (L:vars) (Ψ:denv) (e:exp) (A B:typ) (eᶠ:fexp),
+      d_wf_typ Ψ A ->
+      ( forall x , x \notin  L  -> d_chk_inf_elab  ( x ~ (dbind_typ A)  ++  Ψ )  ( open_exp_wrt_exp e (exp_var_f x) ) typingmode__chk B (open_fexp_wrt_fexp eᶠ (fexp_var_f x)))  ->
+      d_chk_inf_elab Ψ (exp_abs e) typingmode__chk (typ_arrow A B)
+        (fexp_abs (trans_typ A) eᶠ)
+  | d_chk_inf_elab__chk_sub : forall (Ψ:denv) (e:exp) ( A B:typ) (eᶠ co:fexp),
+      d_chk_inf_elab Ψ e typingmode__inf A eᶠ ->
+      d_sub_elab Ψ A B co ->
+      d_chk_inf_elab Ψ e typingmode__chk B
+        (fexp_app co eᶠ)
+  | d_chk_inf_elab__chk_intersection : forall (Ψ:denv) (e:exp) (A1 A2:typ) (e1ᶠ e2ᶠ:fexp),
+      d_chk_inf_elab Ψ e typingmode__chk A1 e1ᶠ ->
+      d_chk_inf_elab Ψ e typingmode__chk A2 e2ᶠ ->
+      d_chk_inf_elab Ψ e typingmode__chk (typ_intersection A1 A2)
+        (fexp_pair e1ᶠ e2ᶠ)
+  | d_chk_inf_elab__chk_union1 : forall (Ψ:denv) (e:exp) (A1 A2:typ) (eᶠ:fexp),
+      d_chk_inf_elab Ψ e typingmode__chk A1 eᶠ ->
+      d_wf_typ Ψ A2 ->
+      d_chk_inf_elab Ψ e typingmode__chk (typ_union A1 A2)
+        (fexp_inl eᶠ)
+  | d_chk_inf_elab__chk_union2 : forall (Ψ:denv) (e:exp) (A1 A2:typ) (eᶠ:fexp),
+      d_chk_inf_elab Ψ e typingmode__chk A2 eᶠ ->
+      d_wf_typ Ψ A1 ->
+      d_chk_inf_elab Ψ e typingmode__chk (typ_union A1 A2)
+        (fexp_inr eᶠ).
+
+
+(* 
+
+
+
+
+Hint Constructors d_sub_elab : safety.
+Hint Constructors typing : safety.
+
+
+
 
 Lemma open_fexp_wrt_fexp_rec_lc_fexp : forall e2 e1 n,
   lc_fexp e2 -> open_fexp_wrt_fexp_rec n e1 e2 = e2.
@@ -257,8 +409,8 @@ Proof.
   apply degree_fexp_wrt_ftyp_of_lc_fexp. auto.
 Qed.
 
-Theorem sub_elab_lc_fexp : forall E A B C,
-  d_sub_elab E A B C -> lc_fexp C.
+Theorem sub_elab_lc_fexp : forall Ψ A B C,
+  d_sub_elab Ψ A B C -> lc_fexp C.
 Proof.
   intros. induction H.
   - eauto with safety.
@@ -330,34 +482,34 @@ Proof.
     rewrite open_fexp_wrt_fexp_rec_lc_fexp; auto.
 Admitted.
 
-Theorem sub_sound_f : forall E A B C,
-  d_sub_elab E A B C -> typing (trans_env E) C (ftyp_arrow (trans_typ A) (trans_typ B)).
+Theorem sub_sound_f : forall Ψ A B C,
+  d_sub_elab Ψ A B C -> typing (trans_env Ψ) C (ftyp_arrow (trans_typ A) (trans_typ B)).
 Proof with eauto with safety.
   intros. induction H; simpl; eauto.
-  - apply typing_abs with (L:=dom E).
+  - apply typing_abs with (L:=dom Ψ).
     unfold open_fexp_wrt_fexp. simpl. intros.
     apply typing_tapp with (B1:=ftyp_var_b 0); eauto with safety.
     apply typing_var; eauto.
     apply wf_env_typ; eauto with safety.
-    apply trans_typ_wf with (E:=E) (T:=typ_all (typ_var_b 0)).
-    apply dwftyp_all with (L:=dom E); unfold open_typ_wrt_typ; simpl; auto.
-  - apply typing_abs with (L:=dom E).
+    apply trans_typ_wf with (Ψ:=Ψ) (T:=typ_all (typ_var_b 0)).
+    apply dwftyp_all with (L:=dom Ψ); unfold open_typ_wrt_typ; simpl; auto.
+  - apply typing_abs with (L:=dom Ψ).
     unfold open_fexp_wrt_fexp. simpl. intros.
     apply typing_var; eauto.
     apply wf_env_typ; eauto with safety.
-  - apply typing_abs with (L:=dom E).
+  - apply typing_abs with (L:=dom Ψ).
     unfold open_fexp_wrt_fexp. simpl. intros.
     apply typing_var; eauto.
     apply wf_env_typ; eauto with safety.
     apply trans_typ_wf with (T:=typ_var_f X); auto.
-  - apply typing_abs with (L:=dom E).
+  - apply typing_abs with (L:=dom Ψ).
     unfold open_fexp_wrt_fexp. simpl. intros.
     apply typing_var; eauto.
     apply wf_env_typ; eauto with safety.
     apply trans_typ_wf with (T:=typ_var_f SX); auto.
-  - apply typing_abs with (L:=dom E).
+  - apply typing_abs with (L:=dom Ψ).
     unfold open_fexp_wrt_fexp. simpl. intros.
-    apply typing_abs with (L:=dom E `union` singleton x).
+    apply typing_abs with (L:=dom Ψ `union` singleton x).
     unfold open_fexp_wrt_fexp. simpl. intros.
     assert (Hlc1: lc_fexp C1).
     { apply sub_elab_lc_fexp in H. auto. }
@@ -374,9 +526,9 @@ Proof with eauto with safety.
       -- admit. (* weaken *)
       -- apply typing_var; auto.
        admit. (* wf *)
-  - apply typing_abs with (L:=L `union` dom E).
+  - apply typing_abs with (L:=L `union` dom Ψ).
     unfold open_fexp_wrt_fexp. simpl. intros.
-    apply typing_tabs with (L:=L `union` dom E `union` singleton x).
+    apply typing_tabs with (L:=L `union` dom Ψ `union` singleton x).
     unfold open_fexp_wrt_ftyp. simpl. intros.
     inst_cofinites_with X.
     assert (Hlc: lc_fexp C).
@@ -393,7 +545,7 @@ Proof with eauto with safety.
     apply typing_tapp; eauto with safety.
     apply typing_var; auto.
     admit. (* wf *)
-  - apply typing_abs with (L:=L `union` dom E).
+  - apply typing_abs with (L:=L `union` dom Ψ).
     unfold open_fexp_wrt_fexp. simpl. intros.
     assert (Hlc: lc_fexp C).
     { apply sub_elab_lc_fexp in H5. auto. }
@@ -405,7 +557,7 @@ Proof with eauto with safety.
     apply typing_tapp; eauto with safety.
     apply typing_var; auto.
     admit. (* wf *)
-  - apply typing_abs with (L:=dom E).
+  - apply typing_abs with (L:=dom Ψ).
     intros. unfold open_fexp_wrt_fexp. simpl.
     assert (Hlc1: lc_fexp C1).
     { apply sub_elab_lc_fexp in H. auto. }
@@ -422,7 +574,7 @@ Proof with eauto with safety.
       * admit. (* weaken *)
       * apply typing_var; auto.
         admit. (* wf *)
-  - apply typing_abs with (L:=dom E).
+  - apply typing_abs with (L:=dom Ψ).
     intros. unfold open_fexp_wrt_fexp. simpl.
     assert (Hlc: lc_fexp C).
     { apply sub_elab_lc_fexp in H. auto. }
@@ -433,7 +585,7 @@ Proof with eauto with safety.
     + apply typing_proj1 with (B2:=trans_typ A2).
     apply typing_var; auto.
     admit. (* wf *)
-  - apply typing_abs with (L:=dom E).
+  - apply typing_abs with (L:=dom Ψ).
     intros. unfold open_fexp_wrt_fexp. simpl.
     assert (Hlc: lc_fexp C).
     { apply sub_elab_lc_fexp in H. auto. }
@@ -444,7 +596,7 @@ Proof with eauto with safety.
     + apply typing_proj2 with (B1:=trans_typ A1).
     apply typing_var; auto.
     admit. (* wf *)
-  - apply typing_abs with (L:=dom E).
+  - apply typing_abs with (L:=dom Ψ).
     intros. unfold open_fexp_wrt_fexp. simpl.
     assert (Hlc: lc_fexp C).
     { apply sub_elab_lc_fexp in H. auto. }
@@ -456,7 +608,7 @@ Proof with eauto with safety.
       * apply typing_var; auto.
         admit. (* wf *)
     + admit. (* wf *)
-  - apply typing_abs with (L:=dom E).
+  - apply typing_abs with (L:=dom Ψ).
     intros. unfold open_fexp_wrt_fexp. simpl.
     assert (Hlc: lc_fexp C).
     { apply sub_elab_lc_fexp in H. auto. }
@@ -468,7 +620,7 @@ Proof with eauto with safety.
       * apply typing_var; auto.
         admit. (* wf *)
     + admit. (* wf *)
-  - apply typing_abs with (L:=dom E).
+  - apply typing_abs with (L:=dom Ψ).
     intros. unfold open_fexp_wrt_fexp. simpl.
     assert (Hlc1: lc_fexp C1).
     { apply sub_elab_lc_fexp in H. auto. }
@@ -477,7 +629,7 @@ Proof with eauto with safety.
     repeat rewrite open_fexp_wrt_fexp_rec_lc_fexp;
     try rewrite open_fexp_wrt_fexp_rec_lc_fexp; auto.
     apply typing_case with (B1:=trans_typ A1) (B2:=trans_typ A2)
-               (L:=dom E `union` singleton x).
+               (L:=dom Ψ `union` singleton x).
     + apply typing_var; auto. admit. (* wf *) 
     + intros. unfold open_fexp_wrt_fexp. simpl.
     rewrite open_fexp_wrt_fexp_rec_lc_fexp; auto.
@@ -493,51 +645,6 @@ Proof with eauto with safety.
         admit. (* wf *) 
 Admitted.
 
-Inductive infabs_elab : denv -> typ -> typ -> typ -> fexp -> Prop := 
-| infabs_elab_bot : forall (E:denv),
-  d_wf_env E ->
-  infabs_elab E typ_bot typ_top typ_bot
-    (fexp_abs (ftyp_all (ftyp_var_b 0))
-          (fexp_tapp (fexp_var_b 0) (ftyp_arrow ftyp_unit (ftyp_all (ftyp_var_b 0)))))
-| infabs_elab_arr : forall (E:denv) (B1 B2:typ),
-  d_wf_env E ->
-  d_wf_typ E B1 ->
-  d_wf_typ E B2 ->
-  infabs_elab E (typ_arrow B1 B2) B1 B2
-    (fexp_abs (trans_typ (typ_arrow B1 B2)) (fexp_var_b 0))
-| infabs_elab_all : forall (E:denv) (B1 B2 T3 T4:typ) (Co:fexp),
-  d_mono_typ B2 -> 
-  d_wf_typ E B2 ->
-  d_wf_typ E (typ_all B1) ->
-  infabs_elab E  (open_typ_wrt_typ  B1   B2 ) T3 T4 Co ->
-  infabs_elab E (typ_all B1) T3 T4
-    (fexp_abs (trans_typ (typ_all B1))
-              (fexp_app Co (fexp_tapp (fexp_var_b 0) (trans_typ B2))))
-| infabs_elab_intersection1 : forall (E:denv) (B1 B2 T3 T4:typ) (Co:fexp),
-  d_wf_typ E B2 ->
-  infabs_elab E B1 T3 T4 Co ->
-  infabs_elab E (typ_intersection B1 B2) T3 T4
-    (fexp_abs (trans_typ (typ_intersection B1 B2))
-              (fexp_app Co (fexp_proj1 (fexp_var_b 0))))
-| infabs_elab_intersection2 : forall (E:denv) (B1 B2 T3 T4:typ) (Co:fexp),
-  d_wf_typ E B1 ->
-  infabs_elab E B2 T3 T4 Co ->
-  infabs_elab E (typ_intersection B1 B2) T3 T4
-    (fexp_abs (trans_typ (typ_intersection B1 B2))
-              (fexp_app Co (fexp_proj2 (fexp_var_b 0))))
-| infabs_elab_union : forall (E:denv) (B1 B2 T3 T4 T5 T6:typ) (Co1 Co2:fexp),
-  infabs_elab E B1 T3 T4 Co1 ->
-  infabs_elab E B2 T5 T6 Co2 ->
-  infabs_elab E (typ_union B1 B2) (typ_intersection T3 T5) (typ_union T4 T6)
-    (fexp_abs (trans_typ (typ_union B1 B2))
-              (fexp_abs (trans_typ (typ_intersection T3 T5))
-                        (fexp_case (fexp_var_b 1)
-                                   (fexp_inl (fexp_app Co1 (fexp_proj1 (fexp_var_b 1))))
-                                   (fexp_inr (fexp_app Co2 (fexp_proj2 (fexp_var_b 1)))))))
-.
-
-Notation "E ⊢ B1 ▹ B2 → T3 ↪ C" :=   (infabs_elab E B1 B2 T3 C) 
-  (at level 65, B1 at next level, B2 at next level, no associativity) : type_scope.
 
 Lemma lc_ftyp_all_id : lc_ftyp (ftyp_all (ftyp_var_b 0)).
 Proof.
@@ -546,8 +653,8 @@ Qed.
 
 Hint Resolve lc_ftyp_all_id : safety.
 
-Theorem infabs_elab_lc_fexp : forall E A B C Co,
-  infabs_elab E A B C Co -> lc_fexp Co.
+Theorem infabs_elab_lc_fexp : forall Ψ A B C Co,
+  infabs_elab Ψ A B C Co -> lc_fexp Co.
 Proof.
   intros. induction H; eauto with safety;
   apply lc_fexp_abs; eauto with safety; simpl.
@@ -559,24 +666,24 @@ Proof.
     rewrite open_fexp_wrt_fexp_rec_lc_fexp; auto.
   - apply lc_ftyp_prod.
     + admit.
-    + apply trans_typ_lc_ftyp. apply d_wf_typ_lc_typ with (E:=E); auto.
+    + apply trans_typ_lc_ftyp. apply d_wf_typ_lc_typ with (Ψ:=Ψ); auto.
   - unfold open_fexp_wrt_fexp. simpl. intros.
     apply lc_fexp_app; eauto with safety.
     rewrite open_fexp_wrt_fexp_rec_lc_fexp; auto.
   - apply lc_ftyp_prod.
-    + apply trans_typ_lc_ftyp. apply d_wf_typ_lc_typ with (E:=E); auto.
+    + apply trans_typ_lc_ftyp. apply d_wf_typ_lc_typ with (Ψ:=Ψ); auto.
     + admit.
   - unfold open_fexp_wrt_fexp. simpl. intros.
     apply lc_fexp_app; eauto with safety.
     rewrite open_fexp_wrt_fexp_rec_lc_fexp; auto.
 Admitted.
 
-Theorem infabs_sound_f : forall E A B C Co,
-  infabs_elab E A B C Co ->
-  typing (trans_env E) Co (ftyp_arrow (trans_typ A) (ftyp_arrow (trans_typ B) (trans_typ C))).
+Theorem infabs_sound_f : forall Ψ A B C Co,
+  infabs_elab Ψ A B C Co ->
+  typing (trans_env Ψ) Co (ftyp_arrow (trans_typ A) (ftyp_arrow (trans_typ B) (trans_typ C))).
 Proof with eauto with safety.
   intros. induction H; simpl; eauto.
-  - apply typing_abs with (L:=dom E).
+  - apply typing_abs with (L:=dom Ψ).
     unfold open_fexp_wrt_fexp. simpl. intros.
     replace (ftyp_arrow ftyp_unit (ftyp_all (ftyp_var_b 0))) with
         (open_ftyp_wrt_ftyp (ftyp_var_b 0)
@@ -585,10 +692,10 @@ Proof with eauto with safety.
     + apply lc_ftyp_arrow; auto.
     apply lc_ftyp_all. unfold open_ftyp_wrt_ftyp. simpl. auto.
     + apply typing_var; auto. admit. (* wf *)
-  - apply typing_abs with (L:=dom E).
+  - apply typing_abs with (L:=dom Ψ).
     unfold open_fexp_wrt_fexp. simpl. intros.
     apply typing_var; auto. admit. (* wf *)
-  - apply typing_abs with (L:=dom E).
+  - apply typing_abs with (L:=dom Ψ).
     unfold open_fexp_wrt_fexp. simpl. intros.
     assert (Hlc: lc_fexp Co).
     { apply infabs_elab_lc_fexp in H2. auto. }
@@ -598,7 +705,7 @@ Proof with eauto with safety.
     + rewrite trans_typ_open_typ_wrt_typ. apply typing_tapp.
       * apply trans_typ_lc_ftyp; auto.
       * apply typing_var; auto. admit. (* wf *)
-  - apply typing_abs with (L:=dom E).
+  - apply typing_abs with (L:=dom Ψ).
     unfold open_fexp_wrt_fexp. simpl. intros.
     assert (Hlc: lc_fexp Co).
     { apply infabs_elab_lc_fexp in H0. auto. }
@@ -607,7 +714,7 @@ Proof with eauto with safety.
     + admit. (* weaken *)
     + apply typing_proj1 with (B2:=trans_typ B2).
       apply typing_var; auto. admit. (* wf *)
-  - apply typing_abs with (L:=dom E).
+  - apply typing_abs with (L:=dom Ψ).
     unfold open_fexp_wrt_fexp. simpl. intros.
     assert (Hlc: lc_fexp Co).
     { apply infabs_elab_lc_fexp in H0. auto. }
@@ -616,18 +723,18 @@ Proof with eauto with safety.
     + admit. (* weaken *)
     + apply typing_proj2 with (B1:=trans_typ B1).
       apply typing_var; auto. admit. (* wf *)
-  - apply typing_abs with (L:=dom E).
+  - apply typing_abs with (L:=dom Ψ).
     unfold open_fexp_wrt_fexp. simpl. intros.
-    assert (Hlc1: lc_fexp Co1).
+    assert (Hlc1: lc_fexp co1).
     { apply infabs_elab_lc_fexp in H. auto. }
-    assert (Hlc2: lc_fexp Co2).
+    assert (Hlc2: lc_fexp co2).
     { apply infabs_elab_lc_fexp in H0. auto. }
     repeat rewrite open_fexp_wrt_fexp_rec_lc_fexp; auto.
-    apply typing_abs with (L:=dom E `union` singleton x).
+    apply typing_abs with (L:=dom Ψ `union` singleton x).
     intros. unfold open_fexp_wrt_fexp. simpl.
     repeat rewrite open_fexp_wrt_fexp_rec_lc_fexp; auto.
     apply typing_case with
-      (L:=dom E `union` singleton x `union` singleton x0)
+      (L:=dom Ψ `union` singleton x `union` singleton x0)
       (B1:=trans_typ B1) (B2:=trans_typ B2).
     + apply typing_var; auto. admit. (* wf *)
     + unfold open_fexp_wrt_fexp. simpl. intros.
@@ -648,61 +755,10 @@ Proof with eauto with safety.
       * admit. (* wf *)
 Admitted.
 
-Inductive inftapp_elab : denv -> typ -> typ -> typ -> fexp -> fexp -> Prop := 
-| inftapp_elab_bot : forall (E:denv) (B1:typ),
-  d_wf_env E -> 
-  d_wf_typ E B1 ->
-  inftapp_elab E typ_bot B1 typ_bot
-    (fexp_abs (ftyp_all (ftyp_var_b 0)) (fexp_var_b 0))
-    (fexp_abs (ftyp_all (ftyp_var_b 0)) (fexp_var_b 0))
-| inftapp_elab_all : forall (E:denv) (B1 B2:typ),
-  d_wf_env E -> 
-  d_wf_typ E (typ_all B1) ->
-  d_wf_typ E B2 ->
-  inftapp_elab E (typ_all B1) B2 (open_typ_wrt_typ  B1   B2 )  
-    (fexp_abs (trans_typ (typ_all B1)) (fexp_var_b 0))
-    (fexp_abs (trans_typ (typ_all B1)) (fexp_tapp (fexp_var_b 0) (trans_typ B2)))
-| inftapp_elab_intersection1 : forall (E:denv) (A1 A2 B C1:typ) (Co1 Co2:fexp),
-  d_wf_typ E A2 ->
-  d_inftapp_false A2 ->
-  inftapp_elab E A1 B C1 Co1 Co2 ->
-  inftapp_elab E (typ_intersection A1 A2) B C1
-    (fexp_abs (trans_typ (typ_intersection A1 A2))
-              (fexp_app Co1 (fexp_proj1 (fexp_var_b 0))))
-    Co2
-| inftapp_elab_intersection2 : forall (E:denv) (A1 A2 B C2:typ) (Co1 Co2:fexp),
-  d_wf_typ E A1 ->
-  d_inftapp_false A1 ->
-  inftapp_elab E A2 B C2 Co1 Co2 ->
-  inftapp_elab E (typ_intersection A1 A2) B C2
-    (fexp_abs (trans_typ (typ_intersection A1 A2))
-              (fexp_app Co1 (fexp_proj2 (fexp_var_b 0))))
-    Co2
-| inftapp_elab_intersection3 : forall (E:denv) (A1 A2 B C1 C2:typ) (Co1 Co2 Co3 Co4:fexp),
-  inftapp_elab E A1 B C1 Co1 Co2 ->
-  inftapp_elab E A2 B C2 Co3 Co4 ->
-  inftapp_elab E (typ_intersection A1 A2) B (typ_intersection C1 C2)
-    (fexp_abs (trans_typ (typ_intersection A1 A2))
-              (fexp_pair (fexp_app Co2 (fexp_app Co1 (fexp_proj1 (fexp_var_b 0))))
-                         (fexp_app Co4 (fexp_app Co3 (fexp_proj2 (fexp_var_b 0))))))
-    (fexp_abs (trans_typ ((typ_intersection C1 C2))) (fexp_var_b 0))
-| inftapp_elab_union : forall (E:denv) (A1 A2 B C1 C2:typ) (Co1 Co2 Co3 Co4:fexp),
-  inftapp_elab E A1 B C1 Co1 Co2 ->
-  inftapp_elab E A2 B C2 Co3 Co4 ->
-  inftapp_elab E (typ_union A1 A2) B (typ_union C1 C2)
-    (fexp_abs (trans_typ (typ_union A1 A2))
-              (fexp_case (fexp_var_b 0)
-                         (fexp_inl (fexp_app Co2 (fexp_app Co1 (fexp_var_b 0))))
-                         (fexp_inr (fexp_app Co4 (fexp_app Co3 (fexp_var_b 0))))))
-    (fexp_abs (trans_typ (typ_union C1 C2)) (fexp_var_b 0))
-.
 
-Notation "E ⊢ B1 ○ B2 ⇒⇒ T3 ↪ C1 | C2" :=
-    (inftapp_elab E B1 B2 T3 C1 C2) 
-      (at level 65, B1 at next level, B2 at next level, no associativity) : type_scope. 
 
-Theorem inftapp_elab_lc_fexp : forall E A B C Co1 Co2,
-  inftapp_elab E A B C Co1 Co2 -> lc_fexp Co1 /\ lc_fexp Co2.
+Theorem inftapp_elab_lc_fexp : forall Ψ A B C co1 co2,
+  d_inftapp_elab Ψ A B C co1 co2 -> lc_fexp co1 /\ lc_fexp co2.
 Proof.
   intros. induction H; eauto with safety; simpl.
   - split; apply lc_fexp_abs; eauto with safety;
@@ -717,24 +773,24 @@ Proof.
       apply lc_fexp_tapp; eauto. apply trans_typ_lc_ftyp. eauto. 
 Admitted.
 
-Theorem inftapp_sound_f : forall E A B C Co1 Co2,
-  inftapp_elab E A B C Co1 Co2 -> exists D,
-  typing (trans_env E) Co1 (ftyp_arrow (trans_typ A) D) /\
-    typing (trans_env E) Co2 (ftyp_arrow D (trans_typ C)).
+Theorem inftapp_sound_f : forall Ψ A B C co1 co2,
+  d_inftapp_elab Ψ A B C co1 co2 -> exists D,
+  typing (trans_env Ψ) co1 (ftyp_arrow (trans_typ A) D) /\
+    typing (trans_env Ψ) co2 (ftyp_arrow D (trans_typ C)).
 Proof with eauto with safety.
   intros. induction H; simpl; eauto.
   - exists (ftyp_all (ftyp_var_b 0)). split.
-    + apply typing_abs with (L:=dom E).
+    + apply typing_abs with (L:=dom Ψ).
       unfold open_fexp_wrt_fexp. simpl. intros.
       apply typing_var; auto. admit. (* wf *)
-    + apply typing_abs with (L:=dom E).
+    + apply typing_abs with (L:=dom Ψ).
       unfold open_fexp_wrt_fexp. simpl. intros.
       apply typing_var; auto. admit. (* wf *)
   - exists (ftyp_all (trans_typ B1)). split.
-    + apply typing_abs with (L:=dom E).  
+    + apply typing_abs with (L:=dom Ψ).  
       unfold open_fexp_wrt_fexp. simpl. intros.
       apply typing_var; auto. admit. (* wf *)
-    + apply typing_abs with (L:=dom E).  
+    + apply typing_abs with (L:=dom Ψ).  
       unfold open_fexp_wrt_fexp. simpl. intros.
       rewrite trans_typ_open_typ_wrt_typ.
       apply typing_tapp.
@@ -742,9 +798,9 @@ Proof with eauto with safety.
       * apply typing_var; auto. admit. (* wf *)
   - inversion IHinftapp_elab. destruct H2.
     exists x. split.
-    + apply typing_abs with (L:=dom E).  
+    + apply typing_abs with (L:=dom Ψ).  
       unfold open_fexp_wrt_fexp. simpl. intros.
-      assert (Hlc: lc_fexp Co1 /\ lc_fexp Co2).
+      assert (Hlc: lc_fexp co1 /\ lc_fexp co2).
       { apply inftapp_elab_lc_fexp in H1. auto. }
       destruct Hlc as [Hlc1 Hlc2].
       rewrite open_fexp_wrt_fexp_rec_lc_fexp; auto.
@@ -755,9 +811,9 @@ Proof with eauto with safety.
     + auto.
   - inversion IHinftapp_elab. destruct H2.
     exists x. split.
-    + apply typing_abs with (L:=dom E).
+    + apply typing_abs with (L:=dom Ψ).
       unfold open_fexp_wrt_fexp. simpl. intros.
-      assert (Hlc: lc_fexp Co1 /\ lc_fexp Co2).
+      assert (Hlc: lc_fexp co1 /\ lc_fexp co2).
       { apply inftapp_elab_lc_fexp in H1. auto. }
       destruct Hlc as [Hlc1 Hlc2].
       rewrite open_fexp_wrt_fexp_rec_lc_fexp; auto.
@@ -769,12 +825,12 @@ Proof with eauto with safety.
   - inversion IHinftapp_elab1. inversion IHinftapp_elab2.
     destruct H1. destruct H2.
     exists (trans_typ (typ_intersection C1 C2)). split.
-    + apply typing_abs with (L:=dom E).
+    + apply typing_abs with (L:=dom Ψ).
       unfold open_fexp_wrt_fexp. simpl. intros.
-      assert (Hlc12: lc_fexp Co1 /\ lc_fexp Co2).
+      assert (Hlc12: lc_fexp co1 /\ lc_fexp co2).
       { apply inftapp_elab_lc_fexp in H. auto. }
       destruct Hlc12 as [Hlc1 Hlc2].
-      assert (Hlc34: lc_fexp Co3 /\ lc_fexp Co4).
+      assert (Hlc34: lc_fexp co3 /\ lc_fexp co4).
       { apply inftapp_elab_lc_fexp in H0. auto. }
       destruct Hlc34 as [Hlc3 Hlc4].
       repeat rewrite open_fexp_wrt_fexp_rec_lc_fexp; auto.
@@ -791,22 +847,22 @@ Proof with eauto with safety.
            ++ admit. (* weaken *)
            ++ apply typing_proj2 with (B1:=trans_typ A1).
               apply typing_var; auto. admit. (* wf *)
-    + apply typing_abs with (L:=dom E).
+    + apply typing_abs with (L:=dom Ψ).
       unfold open_fexp_wrt_fexp. simpl. intros.
       apply typing_var; auto. admit. (* wf *)
   - inversion IHinftapp_elab1. inversion IHinftapp_elab2.
     destruct H1. destruct H2.
     exists (trans_typ (typ_union C1 C2)). split.
-    + apply typing_abs with (L:=dom E).
+    + apply typing_abs with (L:=dom Ψ).
       unfold open_fexp_wrt_fexp. simpl. intros.
-      assert (Hlc12: lc_fexp Co1 /\ lc_fexp Co2).
+      assert (Hlc12: lc_fexp co1 /\ lc_fexp co2).
       { apply inftapp_elab_lc_fexp in H. auto. }
       destruct Hlc12 as [Hlc1 Hlc2].
-      assert (Hlc34: lc_fexp Co3 /\ lc_fexp Co4).
+      assert (Hlc34: lc_fexp co3 /\ lc_fexp co4).
       { apply inftapp_elab_lc_fexp in H0. auto. }
       destruct Hlc34 as [Hlc3 Hlc4].
       repeat rewrite open_fexp_wrt_fexp_rec_lc_fexp; auto.
-      apply typing_case with (L:=dom E `union` singleton x1)
+      apply typing_case with (L:=dom Ψ `union` singleton x1)
         (B1:=trans_typ A1) (B2:=trans_typ A2).
       * apply typing_var; auto. admit. (* wf *)
       * unfold open_fexp_wrt_fexp. simpl. intros.
@@ -827,98 +883,30 @@ Proof with eauto with safety.
               ** admit. (* weaken *)
               ** apply typing_var; auto. admit. (* wf *)
         -- admit. (* wf *)
-    + apply typing_abs with (L:=dom E).
+    + apply typing_abs with (L:=dom Ψ).
       unfold open_fexp_wrt_fexp. simpl. intros.
       apply typing_var; auto. admit. (* wf *)  
 Admitted.
 
 
-Inductive typing_elab : denv -> dexp -> d_typing_mode -> typ -> fexp -> Prop :=
-| typing_elab_infvar : forall (E:denv) (x:expvar) (B1:typ),
-  d_wf_env E ->
-  binds ( x )  ( (dbind_typ B1) ) ( E )  ->
-  typing_elab E (dexp_var_f x) d_typingmode_inf B1
-    (fexp_var_f x)
-| typing_elab_infanno : forall (E:denv) (e:dexp) (B1:typ) (C:fexp),
-  d_wf_typ E B1 ->
-  typing_elab E e d_typingmode_chk B1 C ->
-  typing_elab E  ( (dexp_anno e B1) )  d_typingmode_inf B1
-    C
-| typing_elabinf_unit : forall (E:denv),
-  d_wf_env E ->
-  typing_elab E dexp_unit d_typingmode_inf typ_unit
-    fexp_unit
-| typing_elab_infapp : forall (E:denv) (e1 e2:dexp) (B1 B2 T3:typ) (C1 C2 C3:fexp),
-  typing_elab E e1 d_typingmode_inf B1 C1 ->
-  infabs_elab E B1 B2 T3 C2 ->
-  typing_elab E e2 d_typingmode_chk B2 C3 ->
-  typing_elab E  ( (dexp_app e1 e2) ) d_typingmode_inf T3
-    (fexp_app (fexp_app C2 C1) C3)
-| typing_elab_inftabs : forall (L:vars) (E:denv) (e:dexp) (B1:typ) (C:fexp),
-  d_wf_typ E (typ_all B1) ->
-  ( forall X , X \notin  L  -> typing_elab  ( X ~ dbind_tvar_empty  ++  E ) (dexp_anno  ( open_dexp_wrt_typ e (typ_var_f X) )  ( open_typ_wrt_typ B1 (typ_var_f X) ) ) d_typingmode_chk ( open_typ_wrt_typ B1 (typ_var_f X) ) C)  ->
-  typing_elab E (dexp_tabs (dbody_anno e B1)) d_typingmode_inf (typ_all B1)
-    (fexp_tabs C)
-| typing_elab_inftapp : forall (E:denv) (e1:dexp) (B1 B2 T3:typ) (C1 C2 C3:fexp),
-  d_wf_typ E B2 ->
-  typing_elab E e1 d_typingmode_inf B1 C1 ->
-  inftapp_elab E B1 B2 T3 C2 C3 ->
-  typing_elab E (dexp_tapp e1 B2) d_typingmode_inf T3
-    (fexp_app C3 (fexp_app C2 C1))
-| typing_elab_chkabstop : forall (L:vars) (E:denv) (e:dexp) (C:fexp),
-  ( forall x , x \notin  L  -> typing_elab  ( x ~ (dbind_typ typ_bot)  ++  E )   ( open_dexp_wrt_dexp e (dexp_var_f x) ) d_typingmode_chk typ_top C)  ->
-  typing_elab E (dexp_abs e) d_typingmode_chk typ_top
-    fexp_unit
-| typing_elab_chkabs : forall (L:vars) (E:denv) (e:dexp) (B1 B2:typ) (C:fexp),
-  d_wf_typ E B1 ->
-  ( forall x , x \notin  L  -> typing_elab  ( x ~ (dbind_typ B1)  ++  E )  ( open_dexp_wrt_dexp e (dexp_var_f x) ) d_typingmode_chk B2 C)  ->
-  typing_elab E (dexp_abs e) d_typingmode_chk (typ_arrow B1 B2)
-    (fexp_abs (trans_typ B1) C)
-| typing_elab_chkall : forall (L:vars) (E:denv) (e:dexp) (B1:typ) (C:fexp),
-  d_wf_typ E (typ_all B1) ->
-  ( forall X , X \notin  L  -> typing_elab  ( X ~ dbind_tvar_empty  ++  E )  e  d_typingmode_chk ( open_typ_wrt_typ B1 (typ_var_f X) ) C)  ->
-  typing_elab E e d_typingmode_chk (typ_all B1)
-    (fexp_tabs C)
-| typing_elab_chksub : forall (E:denv) (e:dexp) (B1 A1:typ) (C1 C2:fexp),
-  typing_elab E e d_typingmode_inf A1 C1 ->
-  d_sub_elab E A1 B1 C2 ->
-  typing_elab E e d_typingmode_chk B1
-    (fexp_app C2 C1)
-| typing_elab_chkintersection : forall (E:denv) (e:dexp) (A1 B1:typ) (C1 C2:fexp),
-  typing_elab E e d_typingmode_chk A1 C1 ->
-  typing_elab E e d_typingmode_chk B1 C2 ->
-  typing_elab E e d_typingmode_chk (typ_intersection A1 B1)
-    (fexp_pair C1 C2)
-| typing_elab_chkunion1 : forall (E:denv) (e:dexp) (A1 B1:typ) (C:fexp),
-  typing_elab E e d_typingmode_chk A1 C ->
-  d_wf_typ E B1 ->
-  typing_elab E e d_typingmode_chk (typ_union A1 B1)
-    (fexp_inl C)
-| typing_elab_chkunion2 : forall (E:denv) (e:dexp) (A1 B1:typ) (C:fexp),
-  typing_elab E e d_typingmode_chk B1 C ->
-  d_wf_typ E A1 ->
-  typing_elab E e d_typingmode_chk (typ_union A1 B1)
-    (fexp_inr C)
-.
-
-Theorem trans_binds : forall E x T,
-  binds x (dbind_typ T) E -> binds x (bind_typ (trans_typ T)) (trans_env E).
+Theorem trans_binds : forall Ψ x T,
+  binds x (dbind_typ T) Ψ -> binds x (bind_typ (trans_typ T)) (trans_env Ψ).
 Proof.
-  intros. induction E; auto.
+  intros. induction Ψ; auto.
   inversion H.
   - subst. simpl. auto.
   - apply IHE in H0. destruct a.
     destruct b; simpl; auto.
 Qed.
 
-Theorem typing_elab_lc_fexp : forall E e T C mode,
-  typing_elab E e mode T C -> lc_fexp C.
+Theorem d_chk_inf_elab__lc_fexp : forall Ψ e T C mode,
+  d_chk_inf_elab Ψ e mode T C -> lc_fexp C.
 Proof.
   intros. induction H; eauto with safety; simpl.
 Admitted.
 
-Theorem typing_sound_f : forall E e T C mode,
-  typing_elab E e mode T C -> typing (trans_env E) C (trans_typ T).
+Theorem typing_sound_f : forall Ψ e T C mode,
+  d_chk_inf_elab Ψ e mode T C -> typing (trans_env Ψ) C (trans_typ T).
 Proof.
   intros. induction H; simpl; eauto.
   - apply typing_var; auto. admit. (* wf *)
@@ -926,24 +914,24 @@ Proof.
   - apply typing_app with (B1:=trans_typ B2); auto.
     apply typing_app with (B1:=trans_typ B1); auto.
     apply infabs_sound_f; auto.
-  - apply typing_tabs with (L:=L `union` dom E).
+  - apply typing_tabs with (L:=L `union` dom Ψ).
     unfold open_fexp_wrt_ftyp. simpl. intros.
     inst_cofinites_with X. assert (Hlc: lc_fexp C).
-    { apply typing_elab_lc_fexp in H0. auto. }
+    { apply d_chk_inf_elab__lc_fexp in H0. auto. }
     rewrite open_fexp_wrt_ftyp_rec_lc_fexp; auto.
     rewrite <- trans_typ_open_typ_wrt_typ with (B2:=typ_var_f X). auto.
   - apply inftapp_sound_f in H1. destruct H1. destruct H1.
     apply typing_app with (B1:=x); auto.
     apply typing_app with (B1:=trans_typ B1); auto.
-  - apply typing_abs with (L:=L `union` dom E).
+  - apply typing_abs with (L:=L `union` dom Ψ).
     unfold open_fexp_wrt_ftyp. simpl. intros.
     inst_cofinites_with x. assert (Hlc: lc_fexp C).
-    { apply typing_elab_lc_fexp in H0. auto. }
+    { apply d_chk_inf_elab__lc_fexp in H0. auto. }
     rewrite open_fexp_wrt_fexp_lc_fexp; auto.
-  - apply typing_tabs with (L:=L `union` dom E).
+  - apply typing_tabs with (L:=L `union` dom Ψ).
     unfold open_fexp_wrt_ftyp. simpl. intros.
     inst_cofinites_with X. assert (Hlc: lc_fexp C).
-    { apply typing_elab_lc_fexp in H0. auto. }
+    { apply d_chk_inf_elab__lc_fexp in H0. auto. }
     rewrite open_fexp_wrt_ftyp_rec_lc_fexp; auto.
     rewrite <- trans_typ_open_typ_wrt_typ with (B2:=typ_var_f X). auto.
   - eapply typing_app with (B1:=trans_typ A1); auto.
